Added various Multivariate thoerems, including definitions of "flatten" and "matrify" to convert between matrices and flattened vectors. (These could reasonably be put in the core, but since the only current uses are in the Multivariate theories, they've been put in Multivariate/misc.ml for now.) Added various trivial lemmas about them as well as extending and rationalizing theorems about the Frobenius matrix norm, which now emerges more naturally as the usual Euclidean norm on flattened matrices. New definitions:
        flatten
        matrify

and theorems:

        COMPATIBLE_NORM_FLATTEN
        DOT_FLATTEN
        EXISTS_FLATTEN
        EXISTS_MATRIFY
        FLATTEN_0
        FLATTEN_ADD
        FLATTEN_CMUL
        FLATTEN_COMPONENT
        FLATTEN_EQ
        FLATTEN_EQ_0
        FLATTEN_GSPEC
        FLATTEN_MATRIFY
        FLATTEN_SUB
        FORALL_FLATTEN
        FORALL_MATRIFY
        MATRIFY_0
        MATRIFY_ADD
        MATRIFY_CMUL
        MATRIFY_COMPONENT
        MATRIFY_EQ
        MATRIFY_EQ_0
        MATRIFY_FLATTEN
        MATRIFY_SUB
        NORM_FLATTEN_HADAMARD_LE
        NORM_FLATTEN_MUL_LE
        NORM_FLATTEN_ORTHOGONAL_MATRIX_LMUL
        NORM_FLATTEN_ORTHOGONAL_MATRIX_RMUL
        NORM_FLATTEN_POW_2
        NORM_FLATTEN_TRANSP
        ONORM_LE_NORM_FLATTEN

Multivariate/misc.ml
@@ -202,6 +202,101 @@ let EPSILON_DELTA_MINIMAL = prove
       EXISTS_TAC `(d:A->real) a` THEN ASM_SIMP_TAC[]]]);;
 
 (* ------------------------------------------------------------------------- *)
+(* Converting between matrices/arrays and flattened vectors. We can consider *)
+(* these as curry and uncurry for Cartesian powers.                          *)
+(* ------------------------------------------------------------------------- *)
+
+let flatten = new_definition
+ `(flatten:A^N^M->A^(M,N)finite_prod) =
+        \x. lambda i. x$(1 + (i - 1) DIV dimindex(:N))
+                       $(1 + (i - 1) MOD dimindex(:N))`;;
+
+let matrify = new_definition
+ `(matrify:A^(M,N)finite_prod->A^N^M) =
+        \x. lambda i j. x$((i - 1) * dimindex(:N) + j)`;;
+
+let FLATTEN_COMPONENT = prove
+ (`!m:A^N^M i.
+        1 <= i /\ i <= dimindex(:M) * dimindex(:N)
+        ==> (flatten m)$i = m$(1 + (i - 1) DIV dimindex(:N))
+                             $(1 + (i - 1) MOD dimindex(:N))`,
+  SIMP_TAC[flatten; LAMBDA_BETA; DIMINDEX_FINITE_PROD]);;
+
+let MATRIFY_COMPONENT = prove
+ (`!v:A^(M,N)finite_prod i j.
+        1 <= i /\ i <= dimindex(:M) /\ 1 <= j /\ j <= dimindex(:N)
+        ==> (matrify v)$i$j = v$((i - 1) * dimindex(:N) + j)`,
+  SIMP_TAC[matrify; LAMBDA_BETA]);;
+
+let FLATTEN_MATRIFY = prove
+ (`!a:A^(M,N)finite_prod. flatten(matrify a) = a`,
+  GEN_TAC THEN SIMP_TAC[CART_EQ; flatten; matrify; LAMBDA_BETA] THEN
+  REWRITE_TAC[DIMINDEX_FINITE_PROD] THEN X_GEN_TAC `i:num` THEN STRIP_TAC THEN
+  W(MP_TAC o PART_MATCH (lhand o rand) LAMBDA_BETA o lhand o lhand o snd) THEN
+  REWRITE_TAC[ARITH_RULE `1 <= 1 + x /\ 1 + y <= z <=> y < z`] THEN
+  SIMP_TAC[RDIV_LT_EQ; DIMINDEX_GE_1; LE_1] THEN
+  ANTS_TAC THENL [ASM_ARITH_TAC; DISCH_THEN SUBST1_TAC] THEN
+  W(MP_TAC o PART_MATCH (lhand o rand) LAMBDA_BETA o lhand o snd) THEN
+  REWRITE_TAC[ARITH_RULE `1 <= 1 + x /\ 1 + y <= z <=> y < z`] THEN
+  SIMP_TAC[DIVISION; DIMINDEX_GE_1; LE_1] THEN DISCH_THEN SUBST1_TAC THEN
+  AP_TERM_TAC THEN REWRITE_TAC[ADD_SUB2] THEN
+  MATCH_MP_TAC(ARITH_RULE
+   `1 <= i /\ i - 1 = d * n + m /\ m < n
+     ==> d * n + 1 + m = i`) THEN
+  ASM_REWRITE_TAC[] THEN MATCH_MP_TAC DIVISION THEN
+  SIMP_TAC[DIMINDEX_GE_1; LE_1]);;
+
+let MATRIFY_FLATTEN = prove
+ (`!m:A^N^M. matrify(flatten m) = m`,
+  GEN_TAC THEN SIMP_TAC[CART_EQ; flatten; matrify; LAMBDA_BETA] THEN
+  X_GEN_TAC `i:num` THEN STRIP_TAC THEN
+  X_GEN_TAC `j:num` THEN STRIP_TAC THEN
+  W(MP_TAC o PART_MATCH (lhand o rand) LAMBDA_BETA o lhand o snd) THEN
+  ANTS_TAC THENL
+   [CONJ_TAC THENL [ASM_ARITH_TAC; ALL_TAC] THEN
+    TRANS_TAC LE_TRANS `(i - 1) * dimindex(:N) + dimindex(:N)` THEN
+    ASM_REWRITE_TAC[LE_ADD_LCANCEL] THEN
+    REWRITE_TAC[ARITH_RULE `x * n + n = (x + 1) * n`] THEN
+    ASM_SIMP_TAC[SUB_ADD; DIMINDEX_FINITE_PROD] THEN
+    ASM_SIMP_TAC[LE_MULT_RCANCEL; DIMINDEX_GE_1];
+    DISCH_THEN SUBST1_TAC] THEN
+  REWRITE_TAC[] THEN BINOP_TAC THENL
+   [AP_TERM_TAC; ALL_TAC] THEN
+  MATCH_MP_TAC(ARITH_RULE `1 <= i /\ j = i - 1 ==> 1 + j = i`) THEN
+  ASM_REWRITE_TAC[] THENL
+   [MATCH_MP_TAC DIV_UNIQ THEN EXISTS_TAC `j - 1` THEN ASM_ARITH_TAC;
+    MATCH_MP_TAC MOD_UNIQ THEN EXISTS_TAC `i - 1` THEN ASM_ARITH_TAC]);;
+
+let FORALL_FLATTEN = prove
+ (`!P. (!x. P x) <=> (!x. P(flatten x))`,
+  MESON_TAC[MATRIFY_FLATTEN; FLATTEN_MATRIFY]);;
+
+let FORALL_MATRIFY = prove
+ (`!P. (!x. P x) <=> (!x. P(matrify x))`,
+  MESON_TAC[MATRIFY_FLATTEN; FLATTEN_MATRIFY]);;
+
+let EXISTS_FLATTEN = prove
+ (`!P. (?x. P x) <=> (?x. P(flatten x))`,
+  MESON_TAC[MATRIFY_FLATTEN; FLATTEN_MATRIFY]);;
+
+let EXISTS_MATRIFY = prove
+ (`!P. (?x. P x) <=> (?x. P(matrify x))`,
+  MESON_TAC[MATRIFY_FLATTEN; FLATTEN_MATRIFY]);;
+
+let FLATTEN_GSPEC = prove
+ (`!P:A^N^M->bool. {flatten m | P m} = {v | P(matrify v)}`,
+  REWRITE_TAC[EXTENSION; IN_ELIM_THM] THEN
+  MESON_TAC[FLATTEN_MATRIFY; MATRIFY_FLATTEN]);;
+
+let FLATTEN_EQ = prove
+ (`!m1 m2:real^N^M. flatten m1 = flatten m2 <=> m1 = m2`,
+  MESON_TAC[MATRIFY_FLATTEN]);;
+
+let MATRIFY_EQ = prove
+ (`!m1 m2:real^(M,N)finite_prod. matrify m1 = matrify m2 <=> m1 = m2`,
+  MESON_TAC[FLATTEN_MATRIFY]);;
+
+(* ------------------------------------------------------------------------- *)
 (* A generic notion of "hull" (convex, affine, conic hull and closure).      *)
 (* ------------------------------------------------------------------------- *)
 
